correctness/RegexCorrectness/Regex/Iterators/CapturedGroups.lean
@@ -1,0 +1,48 @@
+-- import Regex.Regex.Captures
+import Regex.Regex.Iterators.CapturedGroups
+import RegexCorrectness.Regex.Basic
+
+open Regex.Data (CaptureGroups)
+open Regex.Strategy (materializeRegexGroups)
+open String (Pos)
+
+namespace Regex.CapturedGroups
+
+theorem lt_of_get_some {self : CapturedGroups} {i s} (h : self.get i = .some s) :
+  2 * i + 1 < self.buffer.size := by
+  simp [get, Option.bind_eq_some_iff] at h
+  have ⟨p₁, eq₁, p₁', eq₁', p₂, eq₂, p₂', eq₂', eq₃⟩ := h
+  simp [Array.getElem?_eq_some_iff] at eq₂
+  have ⟨lt, eq₂⟩ := eq₂
+  exact lt
+
+theorem get_eq_none_of_ge {self : CapturedGroups} {i} (h : 2 * i + 1 ≥ self.buffer.size) :
+  self.get i = .none := by
+  simp [get]
+  intro p₁ eq₁ p₁' eq₁' p₂ eq₂ p₂' eq₂'
+  simp [Array.getElem?_eq_some_iff] at eq₂
+  have ⟨lt, eq₂⟩ := eq₂
+  omega
+
+def materialize (self : CapturedGroups) (groups : CaptureGroups) : Prop :=
+  ∀ i p₁ p₂, (self.get i) = .some ⟨self.haystack, p₁, p₂⟩ ↔ materializeRegexGroups groups i = .some (p₁, p₂)
+
+/--
+`CapturedGroups` conforms to the spec if and only if:
+
+- the haystack can be split into `l`, `m`, and `r` such that `haystack = l ++ m ++ r`
+- `m` starts after `startPos`.
+- there is a regex match starting at `l`, matching the substring `m`, and ending at `r`
+- `CapturedGroups` contains the positions of the capture groups in the match
+  - in particular, the first group corresponds to the positions of the matched substring `m`
+  - the last match of wins in case the same group is captured multiple times
+-/
+def Spec {re : Regex} (s : re.IsSearchRegex) (haystack : String) (startPos : Pos) (self : CapturedGroups) : Prop :=
+  ∃ it it' groups,
+    it.toString = haystack ∧
+    startPos ≤ it.pos ∧
+    s.expr.Captures it it' groups ∧
+    self.get 0 = .some ⟨haystack, it.pos, it'.pos⟩ ∧
+    self.materialize groups
+
+end Regex.CapturedGroups
