correctness/RegexCorrectness/Regex/Utilities.lean
@@ -1,91 +1,149 @@
 import Regex.Regex.Utilities
-import RegexCorrectness.Regex.Matches
-import RegexCorrectness.Regex.Captures
-
-set_option autoImplicit false
+-- import RegexCorrectness.Regex.Matches
+-- import RegexCorrectness.Regex.Captures
+import RegexCorrectness.Regex.Iterators.Captures
 
 open String (Pos)
+open Std.Iterators (Iter IterM)
 
 namespace Regex
 
 variable {re : Regex} {haystack : String}
 
-theorem captures_of_find_some {positions} (h : re.find haystack = .some positions)
+-- theorem captures_of_find_some {positions} (h : re.find haystack = .some positions)
+--   (s : re.IsSearchRegex) :
+--   Matches.Spec s haystack ⟨0⟩ positions := by
+--   simp [Regex.find] at h
+--   have ⟨_, h⟩ := h
+--   have v := Captures.valid_captures haystack s
+--   exact (Matches.captures_of_next?_some h v).2
+
+-- theorem captures_of_mem_findAll.go {m : Matches} {accum : Array Substring}
+--   (v : m.Valid) (inv : ∀ str ∈ accum, ∃ startPos, Matches.Spec v.1 m.haystack startPos str) :
+--   ∀ str ∈ findAll.go m accum, ∃ startPos, Matches.Spec v.1 m.haystack startPos str := by
+--   induction m, accum using findAll.go.induct with
+--   | case1 m accum positions m' next_some? ih =>
+--     -- next match is found
+--     rw [findAll.go, next_some?]
+--     simp
+--     have regex_eq := Matches.regex_eq_of_next?_some next_some?
+--     have haystack_eq := Matches.haystack_eq_of_next?_some next_some?
+--     simp [regex_eq, haystack_eq] at ih
+
+--     have ⟨v', spec⟩ := Matches.captures_of_next?_some next_some? v
+--     have inv' (str : Substring) (mem : str ∈ accum ∨ str = positions) : ∃ startPos, Matches.Spec v.1 m.haystack startPos str := by
+--       cases mem with
+--       | inl mem => exact inv str mem
+--       | inr eq => exact ⟨m.currentPos, eq ▸ spec⟩
+--     exact ih v' inv'
+--   | case2 m accum next_none? =>
+--     -- next match is not found
+--     rw [findAll.go, next_none?]
+--     dsimp
+--     exact inv
+
+-- theorem captures_of_mem_findAll {positions} (mem : positions ∈ re.findAll haystack)
+--   (s : re.IsSearchRegex) :
+--   ∃ startPos, Matches.Spec s haystack startPos positions := by
+--   simp [Regex.findAll] at mem
+--   have v := Matches.vaild_matches haystack s
+--   exact captures_of_mem_findAll.go v (by simp) positions mem
+
+-- theorem captures_of_capture_some {captured} (h : re.capture haystack = .some captured)
+--   (s : re.IsSearchRegex) :
+--   captured.Spec s haystack ⟨0⟩ := by
+--   simp [Regex.capture] at h
+--   have ⟨_, h⟩ := h
+--   have v := Captures.valid_captures haystack s
+--   exact (Captures.captures_of_next?_some h v).2
+
+-- theorem captures_of_mem_captureAll.go {captures : Captures} {accum : Array CapturedGroups}
+--   (v : captures.Valid) (inv : ∀ captured ∈ accum, ∃ startPos, CapturedGroups.Spec v.1 captures.haystack startPos captured) :
+--   ∀ captured ∈ captureAll.go captures accum, ∃ startPos, CapturedGroups.Spec v.1 captures.haystack startPos captured := by
+--   induction captures, accum using captureAll.go.induct with
+--   | case1 captures accum groups captures' next?_some ih =>
+--     -- next capture is found
+--     rw [captureAll.go, next?_some]
+--     simp
+--     have regex_eq := Captures.regex_eq_of_next?_some next?_some
+--     have haystack_eq := Captures.haystack_eq_of_next?_some next?_some
+--     simp [regex_eq, haystack_eq] at ih
+
+--     have ⟨v', spec⟩ := Captures.captures_of_next?_some next?_some v
+--     have inv' (captured : CapturedGroups) (mem : captured ∈ accum ∨ captured = groups) : ∃ startPos, CapturedGroups.Spec v.1 captures.haystack startPos captured := by
+--       cases mem with
+--       | inl mem => exact inv captured mem
+--       | inr eq => exact ⟨captures.currentPos, eq ▸ spec⟩
+--     exact ih v' inv'
+--   | case2 captures accum next?_none =>
+--     -- next capture is not found
+--     rw [captureAll.go, next?_none]
+--     simp
+--     exact inv
+
+#check Std.Iterators.Iter.mem_toList_iff_isPlausibleIndirectOutput
+#check Std.Iterators.Iter.isPlausibleIndirectOutput_of_mem_toList
+#synth Membership Nat (Array Nat)
+
+#check Std.Iterators.Iter.unattach_toArray_attachWith
+
+-- universe u
+-- inductive Iter.IsPlausibleIndirectOutput {α β : Type u} [Std.Iterators.Iterator α Id β] (it : Std.Iterators.Iter (α := α) β) :
+--     β → Prop where
+--   | direct {out : β} : it.IsPlausibleOutput out →
+--       IsPlausibleIndirectOutput it out
+--   | indirect {it' : Std.Iterators.Iter (α := α) β} {out : β} : it'.IsPlausibleSuccessorOf it →
+--       it'.IsPlausibleIndirectOutput out → IsPlausibleIndirectOutput it out
+
+def captures_attach_spec (regex : Regex) (haystack : String) (s : re.IsSearchRegex) :=
+  regex.captures haystack |>.attachWith (fun groups => ∃ startPos, CapturedGroups.Spec s haystack startPos groups) proof
+where
+  proof (groups : CapturedGroups) (h : (regex.captures haystack).IsPlausibleIndirectOutput groups) : ∃ startPos, CapturedGroups.Spec s haystack startPos groups := by
+    -- generalize eq : regex.captures haystack = it at h
+    cases h with
+    | @direct it groups h => sorry
+    | @indirect it' it groups ps pio => sorry
+
+-- theorem spec_of_captures_isPlausibleIndirectOutputAux {re : Regex} {haystack : String} {it : IterM (α := Captures) m CapturedGroups}
+--   {bufferSize groups} [Monad m] (s : re.IsSearchRegex) (v : it.internalState.Valid)
+--   (pis : it.IsPlausibleIndirectSuccessorOf (re.capturesM haystack m bufferSize)) (pio : it.IsPlausibleIndirectOutput groups) :
+--   ∃ startPos, CapturedGroups.Spec s haystack startPos groups := by
+--   induction pio with
+--   | @direct it out pio => sorry
+--   | @indirect it it' out ps pio ih =>
+--     have := (IterM.IsPlausibleIndirectSuccessorOf.single ps).trans pis
+--     simp [IterM.IsPlausibleSuccessorOf] at ps
+--     obtain ⟨step, eq, ps⟩ := ps
+--     simp [Std.Iterators.IterStep.successor] at eq
+--     sorry
+
+theorem spec_of_mem_captureAllAux {re : Regex} {haystack : String} {it : Iter (α := Captures) CapturedGroups} {groups}
+  (s : re.IsSearchRegex) (v : it.internalState.Valid)
+  (pis : it.IsPlausibleIndirectSuccessorOf (re.captures haystack)) (mem : groups ∈ it.toArray) :
+  ∃ startPos, CapturedGroups.Spec s haystack startPos groups := by
+  match eq : it.step with
+  | .yield it' groups' h =>
+    rw [Iter.toArray_eq_match_step, eq] at mem
+    simp at mem
+    cases mem with
+    | inl eq' => sorry
+    | inr mem => exact spec_of_mem_captureAllAux s sorry sorry mem
+  | .skip it' h => exact spec_of_mem_captureAllAux s sorry sorry mem
+  | .done h => sorry
+termination_by it.finitelyManySteps
+
+theorem spec_of_mem_captureAll {groups} (mem : groups ∈ re.captureAll haystack)
   (s : re.IsSearchRegex) :
-  Matches.Spec s haystack ⟨0⟩ positions := by
-  simp [Regex.find] at h
-  have ⟨_, h⟩ := h
-  have v := Captures.valid_captures haystack s
-  exact (Matches.captures_of_next?_some h v).2
-
-theorem captures_of_mem_findAll.go {m : Matches} {accum : Array Substring}
-  (v : m.Valid) (inv : ∀ str ∈ accum, ∃ startPos, Matches.Spec v.1 m.haystack startPos str) :
-  ∀ str ∈ findAll.go m accum, ∃ startPos, Matches.Spec v.1 m.haystack startPos str := by
-  induction m, accum using findAll.go.induct with
-  | case1 m accum positions m' next_some? ih =>
-    -- next match is found
-    rw [findAll.go, next_some?]
-    simp
-    have regex_eq := Matches.regex_eq_of_next?_some next_some?
-    have haystack_eq := Matches.haystack_eq_of_next?_some next_some?
-    simp [regex_eq, haystack_eq] at ih
-
-    have ⟨v', spec⟩ := Matches.captures_of_next?_some next_some? v
-    have inv' (str : Substring) (mem : str ∈ accum ∨ str = positions) : ∃ startPos, Matches.Spec v.1 m.haystack startPos str := by
-      cases mem with
-      | inl mem => exact inv str mem
-      | inr eq => exact ⟨m.currentPos, eq ▸ spec⟩
-    exact ih v' inv'
-  | case2 m accum next_none? =>
-    -- next match is not found
-    rw [findAll.go, next_none?]
-    dsimp
-    exact inv
-
-theorem captures_of_mem_findAll {positions} (mem : positions ∈ re.findAll haystack)
-  (s : re.IsSearchRegex) :
-  ∃ startPos, Matches.Spec s haystack startPos positions := by
-  simp [Regex.findAll] at mem
-  have v := Matches.vaild_matches haystack s
-  exact captures_of_mem_findAll.go v (by simp) positions mem
-
-theorem captures_of_capture_some {captured} (h : re.capture haystack = .some captured)
-  (s : re.IsSearchRegex) :
-  captured.Spec s haystack ⟨0⟩ := by
-  simp [Regex.capture] at h
-  have ⟨_, h⟩ := h
-  have v := Captures.valid_captures haystack s
-  exact (Captures.captures_of_next?_some h v).2
-
-theorem captures_of_mem_captureAll.go {captures : Captures} {accum : Array CapturedGroups}
-  (v : captures.Valid) (inv : ∀ captured ∈ accum, ∃ startPos, CapturedGroups.Spec v.1 captures.haystack startPos captured) :
-  ∀ captured ∈ captureAll.go captures accum, ∃ startPos, CapturedGroups.Spec v.1 captures.haystack startPos captured := by
-  induction captures, accum using captureAll.go.induct with
-  | case1 captures accum groups captures' next?_some ih =>
-    -- next capture is found
-    rw [captureAll.go, next?_some]
-    simp
-    have regex_eq := Captures.regex_eq_of_next?_some next?_some
-    have haystack_eq := Captures.haystack_eq_of_next?_some next?_some
-    simp [regex_eq, haystack_eq] at ih
-
-    have ⟨v', spec⟩ := Captures.captures_of_next?_some next?_some v
-    have inv' (captured : CapturedGroups) (mem : captured ∈ accum ∨ captured = groups) : ∃ startPos, CapturedGroups.Spec v.1 captures.haystack startPos captured := by
-      cases mem with
-      | inl mem => exact inv captured mem
-      | inr eq => exact ⟨captures.currentPos, eq ▸ spec⟩
-    exact ih v' inv'
-  | case2 captures accum next?_none =>
-    -- next capture is not found
-    rw [captureAll.go, next?_none]
-    simp
-    exact inv
-
-theorem captures_of_mem_captureAll {captured} (mem : captured ∈ re.captureAll haystack)
-  (s : re.IsSearchRegex) :
-  ∃ startPos, CapturedGroups.Spec s haystack startPos captured := by
-  simp [Regex.captureAll] at mem
-  have v := Captures.valid_captures haystack s
-  exact captures_of_mem_captureAll.go v (by simp) captured mem
+  ∃ startPos, CapturedGroups.Spec s haystack startPos groups := by
+  dsimp [Regex.captureAll] at mem
+  exact spec_of_mem_captureAllAux s (Captures.valid_captures haystack s) (.refl (re.captures haystack)) mem
+  -- rw [Array.mem_def, Std.Iterators.Iter.toList_toArray] at mem
+  -- have h := Std.Iterators.Iter.isPlausibleIndirectOutput_of_mem_toList mem
+  -- generalize eq : re.captures haystack = it at h
+  -- -- ????
+  -- induction h generalizing re with
+  -- | @direct it groups po => sorry
+  -- | @indirect it' it groups ps pio ih => sorry
+  -- -- exact captures_of_mem_captureAll.go v (by simp) captured mem
 
 end Regex
